Cvc/Smt.lean
@@ -1,5 +1,0 @@
-import Cvc.Defs
-
-
-
-namespace Cvc
